ExecFrameworkIntegration.v
@@ -1,0 +1,366 @@
+Require Import String ZArith.
+From ConCert Require Import TCTranslate ExecFrameworkExamples CustomTactics.
+Require Import List.
+Require Import PeanoNat.
+Require Import Coq.ssr.ssrbool.
+Require Import Morphisms.
+
+From SmartContracts Require Import Blockchain Congress Automation.
+(* From RecordUpdate Require Import RecordUpdate. *)
+Import ListNotations.
+Open Scope list.
+
+Import AcornBlockchain CrowdfundingContract.
+
+Global Program Instance CB : ChainBase :=
+  build_chain_base nat Nat.eqb _ _ _ _ Nat.odd. (* Odd addresses are addresses of contracts :) *)
+Next Obligation.
+  eapply NPeano.Nat.eqb_spec.
+Defined.
+
+Definition to_chain (sc : SimpleChain) : Chain :=
+  let '(Build_chain h s fh ab) := sc in build_chain h s fh ab.
+
+Definition of_chain (c : Chain) : SimpleChain :=
+  let '(build_chain h s fh ab) := c in Build_chain h s fh ab.
+
+Definition to_action_body (sab : SimpleActionBody) : ActionBody :=
+  match sab with
+  | Act_transfer addr x => act_transfer addr x
+  end.
+
+Definition to_contract_call_context (scc : SimpleContractCallContext) : ContractCallContext :=
+  let '(Build_ctx from contr_addr am) := scc in build_ctx from contr_addr am.
+
+Definition of_contract_call_context (cc : ContractCallContext) : SimpleContractCallContext :=
+  let '(build_ctx from contr_addr am) := cc in Build_ctx from contr_addr am.
+
+Definition of_state (st : State_coq) : Z * addr_map * nat * nat * bool * Z :=
+  let '(mkState_coq b d o dl d' g):= st in (b,d,o,dl,d',g).
+
+Definition to_state (p : Z * addr_map * nat * nat * bool * Z) :=
+  let '(b,d,o,dl,d',g) := p in mkState_coq b d o dl d' g.
+
+Lemma of_state_to_state p : of_state (to_state p) = p.
+Proof. now destruct p. Qed.
+
+Lemma to_state_of_state st : to_state (of_state st) = st.
+Proof. now destruct st. Qed.
+
+Import Serializable.
+
+Section Serialize.
+
+  Hint Rewrite to_list_of_list of_list_to_list : hints.
+  Global Program Instance addr_map_serialize : Serializable addr_map :=
+    {| serialize m := serialize (to_list m);
+       deserialize l := option_map of_list (deserialize l); |}.
+  Next Obligation.
+    intros. cbn. rewrite deserialize_serialize. cbn.
+    now autorewrite with hints.
+  Defined.
+
+    Global Program Instance State_serializable : Serializable State_coq :=
+    {| serialize st := serialize (of_state st);
+       deserialize p := option_map to_state (deserialize p); |}.
+  Next Obligation.
+    intros. cbn. rewrite deserialize_serialize. now destruct x.
+  Defined.
+
+  Definition of_msg (msg : Msg_coq) : unit + (unit + unit) :=
+    match msg with
+    | Donate_coq => inl tt
+    | GetFunds_coq => inr (inl tt)
+    | Claim_coq => (inr (inr tt))
+    end.
+
+  Definition to_msg (s : unit + (unit + unit)) : Msg_coq :=
+    match s with
+    | inl _ => Donate_coq
+    | inr (inl _) => GetFunds_coq
+    | inr (inr _) => Claim_coq
+    end.
+
+  Lemma of_msg_to_msg s : of_msg (to_msg s) = s.
+  Proof. destruct s as [ | s'];try destruct s';destruct u;simpl;easy. Qed.
+
+  Lemma to_msg_of_msg msg : to_msg (of_msg msg) = msg.
+  Proof. destruct msg;easy. Qed.
+
+  Global Program Instance Msg_serializable : Serializable Msg_coq :=
+    {| serialize msg := serialize (of_msg msg);
+       deserialize s := option_map to_msg (deserialize s); |}.
+  Next Obligation.
+    intros. cbn. rewrite deserialize_serialize. now destruct x.
+  Defined.
+
+
+End Serialize.
+
+Section Wrappers.
+  Definition Setup := (nat * Z)%type.
+
+  Definition init_wrapper (f : SimpleContractCallContext -> nat -> Z -> State_coq):
+    Chain (BaseTypes:=CB) -> ContractCallContext (BaseTypes:=CB) -> Setup -> option State_coq
+    := fun c cc setup => Some (f (of_contract_call_context cc) (fst setup) (snd setup)).
+
+  Definition wrapped_init
+    : Chain -> ContractCallContext -> Setup -> option State_coq
+    := init_wrapper Init.init.
+
+    Definition receive_wrapper
+             (f : SimpleChain ->
+                  SimpleContractCallContext ->
+                   Msg_coq -> State_coq -> option (State_coq * list SimpleActionBody)) :
+    Chain -> ContractCallContext ->
+    State_coq -> option Msg_coq -> option (State_coq * list ActionBody) :=
+    fun ch cc st msg => match msg with
+                       Some msg' => option_map (fun '(st0,acts) => (st0, map to_action_body acts)) (f (of_chain ch) (of_contract_call_context cc) msg' st)
+                     | None => None
+                     end.
+
+  Definition wrapped_receive
+    : Chain -> ContractCallContext -> State_coq -> option Msg_coq -> option (State_coq * list ActionBody)
+    := receive_wrapper Receive.receive.
+
+End Wrappers.
+
+(* Taken from [Congress], because otherwise it is not visible after import *)
+Ltac solve_contract_proper :=
+  repeat
+    match goal with
+    | [ |- ?x _  = ?x _] => unfold x
+    | [ |- ?x _ _ = ?x _ _] => unfold x
+    | [ |- ?x _ _ _ = ?x _ _ _] => unfold x
+    | [ |- ?x _ _ _ _ = ?x _ _ _ _] => unfold x
+    | [ |- ?x _ _ _ _ = ?x _ _ _ _] => unfold x
+    | [ |- ?x _ _ _ _ _ = ?x _ _ _ _ _] => unfold x
+    | [ |- Some _ = Some _] => f_equal
+    | [ |- pair _ _ = pair _ _] => f_equal
+    | [ |- (if ?x then _ else _) = (if ?x then _ else _)] => destruct x
+    | [ |- match ?x with | _ => _ end = match ?x with | _ => _ end ] => destruct x
+    | [H: ChainEquiv _ _ |- _] => rewrite H in *
+    | _ => subst; auto
+    end.
+
+Import FunctionalExtensionality.
+
+Lemma init_proper :
+  Proper (ChainEquiv ==> eq ==> eq ==> eq) wrapped_init.
+Proof. repeat intro; solve_contract_proper. Qed.
+
+Lemma of_chain_proper :
+  Proper (ChainEquiv ==> eq) of_chain.
+Proof. repeat intro. unfold of_chain. destruct x,y;cbn in *. inversion H.
+       cbn in *;subst. f_equal. now apply functional_extensionality.
+Qed.
+
+Lemma receive_proper :
+  Proper (ChainEquiv ==> eq ==> eq ==> eq ==> eq) wrapped_receive.
+Proof.
+  repeat intro. unfold wrapped_receive,receive_wrapper.
+  subst. destruct y2;auto.
+  f_equal.
+  (* TODO : chnage this to avoid funext *)
+  (* unfold Receive.receive. repeat solve_contract_proper. *)
+  f_equal. destruct x,y;solve_contract_proper;cbn.
+  inversion H.
+  cbn in *;subst. solve_contract_proper. solve_contract_proper. f_equal.
+  now apply functional_extensionality.
+Qed.
+
+Definition cf_contract : Contract Setup Msg_coq State_coq :=
+  build_contract wrapped_init init_proper wrapped_receive receive_proper.
+
+Definition cf_state (env : Environment) (address : Blockchain.Address) : option State_coq :=
+  match (env_contract_states env address) with
+  | Some sv => deserialize sv
+  | None => None
+  end.
+
+Import Lia.
+
+Lemma Current_slot_of_chain_eq ch :
+  Current_slot (of_chain ch) = current_slot ch.
+Proof.
+  now destruct ch.
+Qed.
+
+Theorem crowdfunding_balance_consistent to contract state:
+  reachable to ->
+  env_contracts to contract = Some (cf_contract : WeakContract) ->
+  cf_state to contract = Some state ->
+  consistent_balance (Current_slot (of_chain to)) state.
+Proof.
+  intros Hr Hc Hst.
+  cbn in *.
+  assert (address_is_contract contract = true) as addr_format by now eapply contract_addr_format.
+  unfold reachable in *. destruct Hr as [tr].
+  remember empty_state eqn:eq.
+  revert dependent state. revert dependent contract.
+  induction tr as [ |? ? ? steps IH step];intros contract Hc Ha state Hst; subst;try solve_by_inversion.
+  destruct_chain_step.
+  + (* add new block *)
+    cbn in *. intro H. unfold cf_state in *. rewrite env_eq in Hst. cbn in Hst.
+    rewrite Current_slot_of_chain_eq in *.
+    rewrite_environment_equiv.
+    inversion valid_header.
+    eapply IH;eauto.
+    unfold deadline_passed in *. unfold is_true in *.
+    rewrite Bool.negb_true_iff in *. leb_ltb_to_prop. cbn in *. lia.
+  + (* Step *)
+    remember (chain_state_env prev).
+    destruct_action_eval; subst pre; cbn [eval_tx].
+    * (* Transfer step *)
+      rewrite_environment_equiv.
+      cbn in *. unfold cf_state in *. erewrite contract_states_eq in Hst by eauto.
+      cbn in *.
+      intro H. eapply IH;eauto. rewrite Current_slot_of_chain_eq in *.
+      inversion e2. erewrite current_slot_eq in H by eauto. easy.
+    * (* Deployment *)
+      simpl in *.
+      rewrite_environment_equiv.
+      cbn in *. unfold cf_state in *. erewrite contract_states_eq in Hst by eauto.
+      cbn in *. unfold set_chain_contract_state in Hst.
+      intro H. destruct ((contract =? to)%address) eqn:Heq.
+      ** (* Executing the init method *)
+         replace wc with (cf_contract : WeakContract) in * by congruence.
+         cbn in e3. unfold Init.init in *. cbn in e3.
+         unfold Monads.option_bind in e3.
+         destruct (deserialize setup);tryfalse. inversion e3;subst;clear e3.
+         rewrite deserialize_serialize in Hst. inversion Hst. subst.
+         easy.
+      ** rewrite Current_slot_of_chain_eq in *.
+         inversion e4. erewrite current_slot_eq in H by eauto.
+         cbn in H.
+         eapply IH;eauto.
+    * (* Call *)
+      rewrite_environment_equiv.
+      subst new_acts.
+      destruct (address_eqb_spec contract to).
+      ** (* To our contract, runs the [receive] function *)
+        subst. cbn in *.
+        replace wc with (cf_contract : WeakContract) in * by congruence.
+        cbn in e3.
+        unfold Monads.option_bind in e3.
+        destruct (deserialize prev_state) as [p_local_state | ] eqn:Hps;tryfalse.
+        destruct msg as [serialized_msg | ];tryfalse.
+        destruct (deserialize serialized_msg) as [msg | ];tryfalse.
+        destruct (option_map _ _) eqn:Hopt;tryfalse.
+        destruct p as [local_state actions].
+        inversion e3. subst;clear e3.
+        unfold option_map in Hopt.
+        destruct (Receive.receive _ _ _ _) eqn:Hreceive;tryfalse.
+        destruct p. inversion Hopt. subst. clear Hopt.
+        unfold cf_state in *. erewrite contract_states_eq in Hst by eauto.
+        cbn in *. unfold set_chain_contract_state in Hst.
+        rewrite Nat.eqb_refl in Hst.
+        rewrite deserialize_serialize in Hst. inversion Hst. subst.
+        assert (Hprev_consistent: consistent_balance (Current_slot (of_chain prev)) p_local_state) by
+            (eapply IH;eauto;now rewrite e1).
+        remember (Build_ctx from to _) as ctx.
+
+        (* we use one of the functional correctness properties here *)
+        specialize (contract_backed _ ctx msg _ Hprev_consistent) as Hnew_consistent.
+        destruct Hnew_consistent as [fin [out [Hrun Hcon]]].
+        unfold run in Hrun.
+        remember (Build_chain _ _ _ _) as ch.
+        assert (Hreceive' : Receive.receive (of_chain prev) ctx msg p_local_state = Some (state, l0)).
+        { destruct prev, chain_state_env,env_chain;cbn in *.
+          subst. erewrite receive_blockchain_state;eauto. }
+        rewrite Hreceive' in Hrun. inversion Hrun;subst.
+        rewrite Current_slot_of_chain_eq in *.
+        now rewrite_environment_equiv.
+      ** (* Not to our contract *)
+        cbn in *. unfold cf_state in *. erewrite contract_states_eq in Hst by eauto.
+        cbn in *. unfold set_chain_contract_state in Hst.
+        replace ((contract =? to)%address) with false in Hst by (symmetry;now apply Nat.eqb_neq).
+        rewrite Current_slot_of_chain_eq in *.
+        inversion e5. erewrite current_slot_eq by eauto.
+        cbn in *.
+        eapply IH;eauto.
+  + (* Permute queue *)
+    now rewrite prev_next in *.
+Qed.
+
+Theorem crowdfunding_balance_consistent_done to contract state:
+  reachable to ->
+  env_contracts to contract = Some (cf_contract : WeakContract) ->
+  cf_state to contract = Some state ->
+  consistent_balance_done state.
+Proof.
+  intros Hr Hc Hst.
+  cbn in *.
+  assert (address_is_contract contract = true) as addr_format by now eapply contract_addr_format.
+  unfold reachable in *. destruct Hr as [tr].
+  remember empty_state eqn:eq.
+  revert dependent state. revert dependent contract.
+  induction tr as [ |? ? ? steps IH step];intros contract Hc Ha state Hst; subst;try solve_by_inversion.
+  destruct_chain_step.
+  + (* add new block *)
+    cbn in *. intro H. unfold cf_state in *. rewrite env_eq in Hst. cbn in Hst.
+    rewrite_environment_equiv.
+    inversion valid_header.
+    eapply IH;eauto.
+  + (* Step *)
+    remember (chain_state_env prev).
+    destruct_action_eval; subst pre; cbn [eval_tx].
+    * (* Transfer step *)
+      rewrite_environment_equiv.
+      cbn in *. unfold cf_state in *. erewrite contract_states_eq in Hst by eauto.
+      cbn in *.
+      intro H. eapply IH;eauto.
+    * (* Deployment *)
+      simpl in *.
+      rewrite_environment_equiv.
+      cbn in *. unfold cf_state in *. erewrite contract_states_eq in Hst by eauto.
+      cbn in *. unfold set_chain_contract_state in Hst.
+      intro H. destruct ((contract =? to)%address) eqn:Heq.
+      ** (* Executing the init method *)
+         replace wc with (cf_contract : WeakContract) in * by congruence.
+         cbn in e3. unfold Init.init in *. cbn in e3.
+         unfold Monads.option_bind in e3.
+         destruct (deserialize setup);tryfalse. inversion e3;subst;clear e3.
+         rewrite deserialize_serialize in Hst. inversion Hst. subst.
+         easy.
+      ** eapply IH;eauto.
+    * (* Call *)
+      rewrite_environment_equiv.
+      subst new_acts.
+      destruct (address_eqb_spec contract to).
+      ** (* To our contract, runs the [receive] function *)
+        subst. cbn in *.
+        replace wc with (cf_contract : WeakContract) in * by congruence.
+        cbn in e3.
+        unfold Monads.option_bind in e3.
+        destruct (deserialize prev_state) as [p_local_state | ] eqn:Hps;tryfalse.
+        destruct msg as [serialized_msg | ];tryfalse.
+        destruct (deserialize serialized_msg) as [msg | ];tryfalse.
+        destruct (option_map _ _) eqn:Hopt;tryfalse.
+        destruct p as [local_state actions].
+        inversion e3. subst;clear e3.
+        unfold option_map in Hopt.
+        destruct (Receive.receive _ _ _ _) eqn:Hreceive;tryfalse.
+        destruct p. inversion Hopt. subst. clear Hopt.
+        unfold cf_state in *. erewrite contract_states_eq in Hst by eauto.
+        cbn in *. unfold set_chain_contract_state in Hst.
+        rewrite Nat.eqb_refl in Hst.
+        rewrite deserialize_serialize in Hst. inversion Hst. subst.
+        assert (Hprev_consistent: consistent_balance_done p_local_state) by
+            (eapply IH;eauto;now rewrite e1).
+        remember (Build_ctx from to _) as ctx.
+        remember (Build_chain _ _ _ _) as ch.
+
+        (* we use one of the functional correctness properties here *)
+        specialize (contract_state_consistent ch ctx msg _ Hprev_consistent) as Hnew_consistent.
+        destruct Hnew_consistent as [fin [out [Hrun Hcon]]].
+        unfold run in Hrun.
+        rewrite Hreceive in Hrun. now inversion Hrun;subst.
+      ** (* Not to our contract *)
+        cbn in *. unfold cf_state in *. erewrite contract_states_eq in Hst by eauto.
+        cbn in *. unfold set_chain_contract_state in Hst.
+        replace ((contract =? to)%address) with false in Hst by (symmetry;now apply Nat.eqb_neq).
+        eapply IH;eauto.
+  + (* Permute queue *)
+    now rewrite prev_next in *.
+Qed.
