pcuic/PCUICFacts.v
@@ -17,21 +17,6 @@ Import InterpreterEnvList.
 
 Hint Unfold expr_eval_n expr_eval_i : facts.
 
-Ltac inv_andb H := apply Bool.andb_true_iff in H;destruct H.
-Ltac split_andb := apply Bool.andb_true_iff;split.
-Ltac leb_ltb_to_prop :=
-  try rewrite PeanoNat.Nat.ltb_lt in *;
-  try rewrite PeanoNat.Nat.leb_le in *;
-  try rewrite PeanoNat.Nat.leb_gt in *;
-  try rewrite PeanoNat.Nat.ltb_ge in *.
-
-Ltac prop_to_leb_ltb :=
-  try rewrite <- PeanoNat.Nat.ltb_lt in *;
-  try rewrite <-PeanoNat.Nat.leb_le in *;
-  try rewrite <- PeanoNat.Nat.leb_gt in *;
-  try rewrite <- PeanoNat.Nat.ltb_ge in *.
-
-
 (* An elimination principle that takes into account nested occurrences of expressions
    in the list of branches for [eCase] *)
 Definition expr_elim_case (P : expr -> Type)
