pcuic/PCUICTranslate.v
@@ -1,7 +1,7 @@
 Require Import String List.
 From MetaCoq.PCUIC Require Import PCUICAst PCUICLiftSubst.
 From MetaCoq.Template Require Import BasicAst utils monad_utils.
-Require Import Contraver.Ast.
+Require Import ConCert.Ast.
 
 Module P := PCUICAst.
 Import MonadNotation.
